[ISO-DH]: Use key shares to store tokens.

iso_dh/shared.v
@@ -14,12 +14,15 @@ Unset Printing Implicit Defensive.
 Record sess_info := SessInfo {
   si_init : term;
   si_resp : term;
-  si_key  : term;
+  si_init_share : term;
+  si_resp_share : term;
+  si_secret : term;
   si_time : nat;
 }.
 
 Global Instance sess_info_inhabited : Inhabited sess_info :=
-  populate (SessInfo inhabitant inhabitant inhabitant inhabitant).
+  populate (SessInfo inhabitant inhabitant inhabitant
+              inhabitant inhabitant inhabitant).
 
 Section Verif.
 
@@ -39,16 +42,16 @@ A --> B: g^a; vkA
 B --> A: {g^a; g^b; vkA}@skB
 A --> B: {g^a; g^b; vkB}@skA
 
-g^{nAnB}
+Result: derive_key [vkA; vkB; g^nA; g^nB; g^{nAnB}]
 
 *)
 
 Definition mkkeyshare : val := λ: "k",
   texp (tint #0) "k".
 
-Lemma wp_mkkeyshare (t : term) E :
+Lemma wp_mkkeyshare (t : term) :
   {{{ True }}}
-    mkkeyshare t @ E
+    mkkeyshare t
   {{{ RET (repr (TExp (TInt 0) t)); True : iProp}}}.
 Proof.
 iIntros "%Φ _ Hpost". wp_lam.
@@ -60,51 +63,59 @@ Qed.
 Definition iso_dh_pred t : iProp :=
   ⌜length (exps t) = 1⌝.
 
+Definition si_key si :=
+  Spec.derive_key
+    (Spec.of_list [TKey Open (si_init si);
+                   TKey Open (si_resp si);
+                   si_init_share si;
+                   si_resp_share si;
+                   si_secret si]).
+
 Definition session_fail si : iProp :=
   public_at (si_time si) (TKey Seal (si_init si)) ∨
   public_at (si_time si) (TKey Seal (si_resp si)).
 
 Definition session si : iProp :=
   ◯Ph (si_time si) ∗
-  term_meta (si_key si) (nroot.@"info")
-    (TKey Open (si_init si), TKey Open (si_resp si), si_time si).
+  term_meta (si_key si) (nroot.@"info") (si_time si).
 
 Lemma session_agree si1 si2 :
   si_key si1 = si_key si2 →
   session si1 -∗ session si2 -∗ ⌜si1 = si2⌝.
 Proof.
-case: si1 si2 => [kI1 kR1 kS n1] [kI2 kR2 _ n2] /= <-.
+case: si1 si2 => [kI1 kR1 ga1 gb1 gab1 n1] [kI2 kR2 ga2 gb2 gab2 n2] /=.
+case/Spec.tag_inj => _.
+case/Spec.of_list_inj => <- <- <- <- <-.
 iIntros "[#hon1 #meta1] [#hon2 #meta2] /=".
-iPoseProof (term_meta_agree with "meta1 meta2") as "%e".
-by case: e => <- <- <-.
+by iPoseProof (term_meta_agree with "meta1 meta2") as "->".
 Qed.
 
 Definition msg2_pred kR m2 : iProp :=
   ∃ ga b vkI n,
+    let vkR := TKey Open kR in
     let gb := TExp (TInt 0) b in
     let gab := TExp ga b in
-    let secret := Spec.derive_key (Spec.of_list [ga; gb; gab]) in
+    let secret := Spec.of_list [vkI; vkR; ga; gb; gab] in
+    let key := Spec.derive_key secret in
     ⌜m2 = Spec.of_list [ga; gb; vkI]⌝ ∗
     minted_at n ga ∗
     (public b ↔ ▷ □ ((∃ kI, ⌜vkI = TKey Open kI⌝ ∗ public_at n (TKey Seal kI)) ∨
                      public_at n (TKey Seal kR))) ∗
     (∀ t, dh_pred b t ↔ ▷ □ iso_dh_pred t) ∗
-    escrow cryptisN
-      (term_token ga ⊤)
-      (term_token secret (↑nroot.@"client")) ∗
-    term_meta secret (nroot.@"info") (vkI, TKey Open kR, n).
+    term_meta key (nroot.@"info") n.
 
 Definition msg3_pred kI m3 : iProp :=
   ∃ a gb kR n,
+    let vkI := TKey Open kI in
+    let vkR := TKey Open kR in
     let ga := TExp (TInt 0) a in
     let gab := TExp gb a in
-    let secret := Spec.derive_key (Spec.of_list [ga; gb; gab]) in
-    ⌜m3 = Spec.of_list [ga; gb; TKey Open kR]⌝ ∗
+    let si := SessInfo kI kR ga gb gab n in
+    ⌜m3 = Spec.of_list [ga; gb; vkR]⌝ ∗
     (public a ↔ ▷ □ (public_at n (TKey Seal kI) ∨
                      public_at n (TKey Seal kR))) ∗
     (∀ t, dh_pred a t ↔ ▷ □ iso_dh_pred t) ∗
-    (public_at n (TKey Seal kR) ∨
-     term_meta secret (nroot.@"info") (TKey Open kI, TKey Open kR, n)).
+    (public_at n (TKey Seal kR) ∨ term_meta (si_key si) (nroot.@"info") n).
 
 Definition iso_dh_ctx : iProp :=
   seal_pred (N.@"m2") msg2_pred ∗
