iso_dh/initiator.v
@@ -35,7 +35,7 @@ Definition initiator : val := λ: "c" "skI" "vkR",
   list_match: ["ga'"; "gb"; "vkI'"] := "m2" in
   guard: eq_term "ga" "ga'" && eq_term "vkI" "vkI'" in
   let: "gab" := texp "gb" "a" in
-  let: "secret" := term_of_list ["ga"; "gb"; "gab"] in
+  let: "secret" := term_of_list ["vkI"; "vkR"; "ga"; "gb"; "gab"] in
   let: "m3" := sign (N.@"m3") "skI" (term_of_list ["ga"; "gb"; "vkR"]) in
   send "c" "m3";;
   SOME (derive_key "secret").
@@ -53,20 +53,26 @@ Lemma wp_initiator c kI kR dq n :
     initiator c kI (TKey Open kR)
   {{{ okS, RET (repr okS);
       ●Ph{dq} n ∗
-      if okS is Some kS then
-        let si := SessInfo kI kR kS n in
+      if okS is Some kS then ∃ si,
+        ⌜si_init si = kI⌝ ∗
+        ⌜si_resp si = kR⌝ ∗
+        ⌜si_key si = kS⌝ ∗
+        ⌜si_time si = n⌝ ∗
         minted kS ∗
         □ (∀ kt, public (TKey kt kS) ↔ ▷ session_fail si) ∗
-        (session_fail si ∨ session si ∗ term_token kS (↑nroot.@"client"))
+        term_token (si_init_share si) ⊤ ∗
+        (session_fail si ∨ session si)
       else True
  }}}.
 Proof.
 rewrite /initiator.
+set vkI := TKey Open kI.
+set vkR := TKey Open kR.
 iIntros "#chan_c #ctx #(? & ?) #p_kI #p_kR %Ψ !> phase Hpost".
 iMod (minted_at_list with "[] phase") as "[phase list]" => //; eauto.
 wp_pures.
 iDestruct "list" as "(%M & #m_M & #minted_at_M)".
-wp_apply wp_vkey. wp_pures.
+wp_apply wp_vkey. wp_pures. rewrite -/vkI.
 wp_bind (mknonce _).
 iApply (wp_mknonce_freshN M
           (λ _, public_at n (TKey Seal kI) ∨
@@ -77,14 +83,15 @@ iApply (wp_mknonce_freshN M
 - iIntros "%a". rewrite big_sepS_singleton minted_TExp minted_TInt /=.
   iIntros "!>"; iSplit; eauto.
   by iIntros "(_ & ?)".
-iIntros "%a %fresh %nonce #m_a #p_a #a_pred token".
+iIntros "%a %fresh %nonce #m_a #s_a #a_pred token".
+set ga := TExp (TInt 0) a.
 rewrite big_sepS_singleton.
 iPoseProof (phase_auth_frag with "phase") as "#phaseI".
-wp_pures. wp_bind (mkkeyshare _). iApply wp_mkkeyshare => //.
-iIntros "!> _". wp_pures. wp_list. wp_term_of_list.
+wp_pures. wp_apply wp_mkkeyshare => //. rewrite -/ga.
+iIntros "_". wp_pures. wp_list. wp_term_of_list.
 wp_pure _ credit:"H1".
 wp_pure _ credit:"H2".
-iAssert (public (TExp (TInt 0) a)) as "p_ga".
+iAssert (public ga) as "p_ga".
 { iApply public_TExp_iff; eauto.
   rewrite minted_TInt.
   iRight. do 2![iSplit => //].
@@ -114,7 +121,8 @@ rewrite minted_TSeal minted_tag minted_of_list /=.
 iDestruct "m_m2" as "(_ & _ & m_gb & _)".
 wp_pures. wp_bind (texp _ _). iApply wp_texp.
 wp_pures. wp_list. wp_term_of_list. wp_pures.
-set seed := Spec.of_list [TExp (TInt 0) a; gb; TExp gb a].
+set gab := TExp gb a.
+set seed := Spec.of_list [vkI; vkR; ga; gb; gab].
 set secret := Spec.derive_key seed.
 wp_pures. wp_list. wp_term_of_list. wp_apply wp_sign. wp_pures.
 iAssert ( |={⊤}=>
@@ -124,19 +132,17 @@ iAssert ( |={⊤}=>
      ⌜gb = TExp (TInt 0) b⌝ ∗
      □ (public b ↔ ▷ □ (public_at n (TKey Seal kI) ∨
                         public_at n (TKey Seal kR))) ∗
-     term_meta secret (nroot.@"info") (TKey Open kI, TKey Open kR, n) ∗
-     term_token secret (↑nroot.@"client")))%I
-  with "[phase token H3]"
+     term_meta secret (nroot.@"info") n))%I
+  with "[phase H3]"
   as "{p_m2} > (phase & p_m2)".
 { iPoseProof (public_TSealE with "p_m2 [//]") as "{p_m2} p_m2".
   iDestruct "p_m2" as "[[comp _]  | (#i_m2 & _ & _)]".
-  { iMod (public_atI with "[ctx] [H3] [phase] [comp]")
-      as "[phase #comp']" => //; try solve_ndisj.
-    iFrame. eauto. }
+  { by iMod (public_atI with "[ctx] [H3] [phase] [comp]")
+      as "[phase #comp']" => //; try solve_ndisj. }
   iMod (lc_fupd_elim_later_pers with "H3 i_m2") as "{i_m2} #i_m2".
   iDestruct "i_m2"
-    as "(%ga & %b & %kI' & %n' & %e_m2 & m_ga & s_b & _ & escrow & pred_b)".
-  case/Spec.of_list_inj: e_m2 => <- -> <- {ga gb kI'} in seed secret *.
+    as "(%ga' & %b & %kI' & %n' & %e_m2 & m_ga & s_b & pred_b & meta)".
+  case/Spec.of_list_inj: e_m2 => <- -> <- {ga' gb kI'} in gab seed secret *.
   case: (decide (n' < n)) => [contra|?].
   { iPoseProof ("minted_at_M" with "[//] m_ga") as "%ga_M".
     move/(_ _ ga_M)/subtermsP: fresh.
@@ -146,8 +152,7 @@ iAssert ( |={⊤}=>
   iPoseProof (minted_at_phase_frag with "m_ga") as "#phaseR".
   iPoseProof (phase_auth_frag_agree with "phase phaseR") as "%".
   have ? : n' = n by lia. subst n'.
-  iMod (escrowE with "escrow token") as ">token" => //.
-  rewrite /secret /seed !TExp_TExpN TExpC2. iFrame.
+  rewrite /secret /seed /gab !TExp_TExpN TExpC2. iFrame.
   iModIntro. iRight. iExists b. iFrame.
   iSplit => //.
   iSplit => //.
@@ -166,48 +171,46 @@ iAssert (public m3) as "#p_m3".
   - by rewrite !public_minted !minted_TKey.
   - iExists a, gb, kR, n. do 3![iSplitR => //].
     iDestruct "p_m2" as "[#?|p_m2]"; eauto.
-    iDestruct "p_m2" as "(%b & % & #? & #? & _)".
+    iDestruct "p_m2" as "(%b & % & #? & #?)".
     iRight. by eauto.
   - rewrite minted_of_list /= minted_TExp /= minted_TInt minted_TKey.
     rewrite !public_minted !minted_TKey. by do ![iSplitL => //].
   - iIntros "!> _".
     rewrite public_of_list /=.
     by do ![iSplit => //]. }
-wp_pures. wp_bind (send _ _). iApply wp_send => //.
+wp_pures. wp_apply wp_send => //.
 wp_pures. wp_bind (derive_key _). iApply wp_derive_key.
-pose si := SessInfo kI kR secret n.
+pose si := SessInfo kI kR ga gb gab n.
 iAssert (minted seed) as "#m_seed".
-{ rewrite minted_of_list /= minted_TExp /= minted_TInt.
-  do !iSplit => //.
-  by iApply minted_TExp => //; iSplit. }
+{ rewrite minted_of_list /= !minted_TExp /= minted_TInt.
+  by do !iSplit => //; iApply public_minted. }
 iAssert (□ (◇ public seed ↔ ▷ session_fail si))%I as "#s_sec".
 { iSplitL; last first.
   { iIntros "!> #comp".
     rewrite public_of_list /=. do !iSplit => //.
     iModIntro. iApply public_TExp => //.
-    iApply "p_a". eauto. }
+    iApply "s_a". eauto. }
   iDestruct "p_m2" as "[#?|p_m2]".
   { iIntros "!> _ !>". by iRight. }
-  iDestruct "p_m2" as "(%b & -> & #p_b & #p_m2 & _)".
+  iDestruct "p_m2" as "(%b & -> & #s_b & #p_m2)".
   iIntros "!> #>p_sk".
-  rewrite TExp_TExpN in seed secret si *.
+  rewrite TExp_TExpN in gab seed secret si *.
   rewrite /secret /seed public_of_list /= public_TExp2_iff; eauto.
-  iDestruct "p_sk" as "(_ & _ & p_sk & _)".
+  iDestruct "p_sk" as "(_ & _ & _ & _ & p_sk & _)".
   iDestruct "p_sk" as "[[_ #p_b'] | [[_ p_a'] | (_ & a_pred' & _)]]".
-  + iPoseProof ("p_b" with "p_b'") as "{p_b} p_b". by eauto.
-  + iPoseProof ("p_a" with "p_a'") as "hon'". by eauto.
+  + iPoseProof ("s_b" with "p_b'") as "p_b". by eauto.
+  + iPoseProof ("s_a" with "p_a'") as "p_a". by eauto.
   + iPoseProof ("a_pred" with "a_pred'") as ">%contra".
     by rewrite exps_TExpN in contra. }
 wp_pures. iApply ("Hpost" $! (Some secret)). iFrame.
-rewrite -[SessInfo _ _ _ _]/si.
-iSplitR => //; first by rewrite minted_derive_key.
-iSplitR => //.
-{ iIntros "!> !> %kt".
+iExists si. iFrame. do !iSplitR => //.
+- by rewrite minted_derive_key.
+- iIntros "!> !> %kt".
   iApply (bi.iff_trans _ (◇ public seed)). iSplit => //.
-  by iApply public_key_derive_key. }
+  by iApply public_key_derive_key.
 iDestruct "p_m2" as "[#fail|p_m2]".
 { iLeft. by iRight. }
-iDestruct "p_m2" as "(%b & -> & #p_b & #p_m2 & token)".
+iDestruct "p_m2" as "(%b & -> & #p_b & #p_m2)".
 iRight. iFrame. iModIntro. by iSplit.
 Qed.
 
